ctx: Namespace changes

Hybrid/Language/Context.lean
@@ -1,5 +1,7 @@
 import Hybrid.Language.Form
 
+namespace FormL
+
 /--
   As opposed to matching logic, here contexts have no "holes".
 
@@ -7,14 +9,17 @@ import Hybrid.Language.Form
 
   Note also that we do not yet apply any modal operator to said argument list.
 -/
-inductive FormL.Context {symbs : Symbols α} {s : symbs.signature.S} (φ : Form symbs s) : FormL symbs sorts → Type u
+inductive Context {symbs : Symbols α} {s : symbs.signature.S} (φ : Form symbs s) : FormL symbs sorts → Type u
   | refl : Context φ φ
   | head : Context φ (.cons φ ψ)
   | tail : Context φ ψ → Context φ (.cons χ ψ)
+
+namespace Context
+
 /--
   Given a `Context φ ψ`, returns the `FormL` obtained by substituting `φ` in `ψ` by a plug.
 -/
-def FormL.Context.subst {φ : Form sig s}
+def subst {φ : Form sig s}
           {ψ : FormL sig sorts} :
     Context φ ψ → Form sig s → FormL sig sorts
   | .refl => id
@@ -23,7 +28,7 @@ def FormL.Context.subst {φ : Form sig s}
   | @Context.tail _ _ _ _ _ _ _  _ h inner_ctx =>
         λ plug => h.cons (inner_ctx.subst plug)
 
-notation:max C:49 "[" φ:50 "]" => FormL.Context.subst C φ
+notation:max C:49 "[" φ:50 "]" => subst C φ
 
 
 /--
@@ -33,31 +38,31 @@ notation:max C:49 "[" φ:50 "]" => FormL.Context.subst C φ
 -/
 
 /-
-def FormL.Context.index {φ : Form symbs s} {ψ : FormL symbs sorts}: φ.Context ψ → Fin (sorts.length)
+def index {φ : Form symbs s} {ψ : FormL symbs sorts}: φ.Context ψ → Fin (sorts.length)
   | .refl => Fin.mk 0 (by simp only [List.length_singleton, Nat.lt_succ_self])
   | .head => Fin.mk 0 (by simp only [List.length_cons, Nat.lt_add_left_iff_pos, Nat.zero_lt_succ])
-  | @FormL.Context.tail _ _ _ _ _ sorts' ψ' _ _ ctx' => Fin.mk (1 + ctx'.index.val) (by
+  | @tail _ _ _ _ _ sorts' ψ' _ _ ctx' => Fin.mk (1 + ctx'.index.val) (by
           have := ctx'.index.isLt
           simp only [List.length_cons, Nat.lt_succ] at this ⊢
           rw [Nat.add_comm]
           exact Nat.add_le_add_right this 1
       )
 
-def FormL.Context.from_index {φ : Form symbs s} {ψ : FormL symbs sorts} : Fin (sorts.length) → Option (φ.Context ψ)
+def from_index {φ : Form symbs s} {ψ : FormL symbs sorts} : Fin (sorts.length) → Option (φ.Context ψ)
   | ⟨0, h⟩ => sorry
   | ⟨n+1, h⟩ => sorry
 -/
 
-def FormL.Context.index {φ : Form symbs s} {ψ : FormL symbs sorts}: φ.Context ψ → Nat
+def index {φ : Form symbs s} {ψ : FormL symbs sorts}: φ.Context ψ → Nat
   | .refl => 0
   | .head => 0
   | .tail ctx' => 1 + ctx'.index
 
-def FormL.Context.from_index {φ : Form symbs s} {ψ : FormL symbs sorts} : Nat → Option (φ.Context ψ)
+def from_index {φ : Form symbs s} {ψ : FormL symbs sorts} : Nat → Option (φ.Context ψ)
   | 0   => sorry
   | n+1 => sorry
 
-def FormL.Context.iso {φ : Form symbs s} {ψ : Form symbs s'} {χ τ : FormL symbs sorts} (C₁ : φ.Context χ) (C₂ : ψ.Context τ) : Prop :=
+def iso {φ : Form symbs s} {ψ : Form symbs s'} {χ τ : FormL symbs sorts} (C₁ : φ.Context χ) (C₂ : ψ.Context τ) : Prop :=
   match C₁ with
   | .refl =>
       match C₂ with
@@ -71,24 +76,28 @@ def FormL.Context.iso {φ : Form symbs s} {ψ : Form symbs s'} {χ τ : FormL sy
       | .tail ctx' => ctx.iso ctx'
       | _ => False
 
-def FormL.subst_to_ctx (χ : Form sig s)
+lemma iso_trans {φ : Form symbs s} {ψ : Form symbs s'} {χ : Form symbs s''} {a b c : FormL symbs sorts} {C₁ : φ.Context a} {C₂ : ψ.Context b} {C₃ : χ.Context c} : C₁.iso C₂ → C₁.iso C₃ → C₂.iso C₃ := sorry
+
+lemma if_iso {φ ψ : Form symbs s} {τ : FormL symbs sorts} (C₁ : φ.Context τ) (C₂ : ψ.Context τ) (h : C₁.iso C₂) : φ = ψ := sorry
+
+lemma if_iso_sorts {φ : Form symbs s} {ψ : Form symbs s'} {τ : FormL symbs sorts} (C₁ : φ.Context τ) (C₂ : ψ.Context τ) (h : C₁.iso C₂) : s = s' := sorry
+
+lemma iso_subst {φ ψ χ : Form symbs s} {τ : FormL symbs sorts} {C₁ : φ.Context τ} {C₂ : ψ.Context C₁[χ]} (h : C₁.iso C₂) : ψ = χ := sorry
+
+lemma iso_subst_sorts {φ χ : Form symbs s} {ψ : Form symbs s'} {τ : FormL symbs sorts} {C₁ : φ.Context τ} {C₂ : ψ.Context C₁[χ]} (h : C₁.iso C₂) : s = s' := sorry
+
+def subst_iso {φ ψ : Form symbs s} {χ : FormL symbs sorts} {C₁ : φ.Context χ} (C₂ : ψ.Context C₁[ψ]) (h : C₁.iso C₂) : (τ : Form symbs s) → Σ' C₃ : τ.Context C₁[τ], C₂.iso C₃ := sorry
+
+def subst_not_iso {φ χ : Form symbs s} {ψ : Form symbs s'} {τ : FormL symbs sorts} {C₁ : φ.Context τ} (C₂ : ψ.Context C₁[χ]) (h : ¬C₁.iso C₂) : (δ : Form symbs s) → Σ' C₃ : ψ.Context C₁[δ], C₂.iso C₃ := sorry
+
+def subst_not_iso' {φ : Form symbs s} {ψ : Form symbs s'} {τ : FormL symbs sorts} {C₁ : φ.Context τ} (C₂ : ψ.Context τ) (h : ¬C₁.iso C₂) : (δ : Form symbs s) → Σ' C₃ : ψ.Context C₁[δ], C₂.iso C₃ := sorry
+
+end Context
+
+def subst_to_ctx (χ : Form sig s)
           {φ : Form sig s}
           {ψ : FormL sig sorts}
           (C : Context φ ψ) :
           χ.Context C[χ] := sorry
 
-lemma FormL.Context.iso_trans {φ : Form symbs s} {ψ : Form symbs s'} {χ : Form symbs s''} {a b c : FormL symbs sorts} {C₁ : φ.Context a} {C₂ : ψ.Context b} {C₃ : χ.Context c} : C₁.iso C₂ → C₁.iso C₃ → C₂.iso C₃ := sorry
-
-lemma FormL.Context.if_iso {φ ψ : Form symbs s} {τ : FormL symbs sorts} (C₁ : φ.Context τ) (C₂ : ψ.Context τ) (h : C₁.iso C₂) : φ = ψ := sorry
-
-lemma FormL.Context.if_iso_sorts {φ : Form symbs s} {ψ : Form symbs s'} {τ : FormL symbs sorts} (C₁ : φ.Context τ) (C₂ : ψ.Context τ) (h : C₁.iso C₂) : s = s' := sorry
-
-lemma FormL.Context.iso_subst {φ ψ χ : Form symbs s} {τ : FormL symbs sorts} {C₁ : φ.Context τ} {C₂ : ψ.Context C₁[χ]} (h : C₁.iso C₂) : ψ = χ := sorry
-
-lemma FormL.Context.iso_subst_sorts {φ χ : Form symbs s} {ψ : Form symbs s'} {τ : FormL symbs sorts} {C₁ : φ.Context τ} {C₂ : ψ.Context C₁[χ]} (h : C₁.iso C₂) : s = s' := sorry
-
-def FormL.Context.subst_iso {φ ψ : Form symbs s} {χ : FormL symbs sorts} {C₁ : φ.Context χ} (C₂ : ψ.Context C₁[ψ]) (h : C₁.iso C₂) : (τ : Form symbs s) → Σ' C₃ : τ.Context C₁[τ], C₂.iso C₃ := sorry
-
-def FormL.Context.subst_not_iso {φ χ : Form symbs s} {ψ : Form symbs s'} {τ : FormL symbs sorts} {C₁ : φ.Context τ} (C₂ : ψ.Context C₁[χ]) (h : ¬C₁.iso C₂) : (δ : Form symbs s) → Σ' C₃ : ψ.Context C₁[δ], C₂.iso C₃ := sorry
-
-def FormL.Context.subst_not_iso' {φ : Form symbs s} {ψ : Form symbs s'} {τ : FormL symbs sorts} {C₁ : φ.Context τ} (C₂ : ψ.Context τ) (h : ¬C₁.iso C₂) : (δ : Form symbs s) → Σ' C₃ : ψ.Context C₁[δ], C₂.iso C₃ := sorry
+end FormL
